\section{Laplace equation in two dimensions}
In this section, we will solve the two-dimensional Laplace equation on a quadratic domain
\begin{equation}
    u_{xx} + u_{yy} = 0, \, (x,y) \in \Omega := [0,1]^2,
    \label{ex3:eq:laplace}
\end{equation}
with boundary conditions on the edges of $\Omega$
\begin{equation*}
    \begin{split}
        u(0,y) &= 0,\\
        u(1,y) &= 0,\\
        u(x,0) &= 0,\\
        u(x,1) &= \sin(2\pi x).\\
    \end{split}
\end{equation*}
We will solve this equation numerically using a five point stencil, but first, we solve it analytically to provide a reference solution which can be compared with the numerical one.

The solution of equation \ref{ex3:eq:laplace} can be found by separation of variables.
First, asssume that we can write
\begin{equation*}
    % I used these names, but I think it's more common with capital X and Y or something.
    % I'm open for discussions of this.
    u(x,y) = \alpha(x) \beta(y),
\end{equation*}
which implies that
\begin{equation*}
    u_{xx} + u_{yy} =  \alpha''(x) \beta(y) + \alpha(x) \beta''(y) = 0,
\end{equation*}
where the prime markers $'$ denote differentiation of the single variable functions $\alpha(x)$ and $\beta(y)$.
Rearranging, we get that
\begin{equation*}
    \frac{\alpha''(x)}{\alpha(x) = \frac{\beta''(y)}{\beta(y)}} = c
\end{equation*}
must be constant, since $\alpha$ and $\beta$ are independent functions.
Thus, we have two second order differential equations
\begin{equation*}
    \begin{split}
        \alpha''(x) - c\alpha(x) &= 0, \\
        \beta''(x) - c\beta(x) &= 0,
    \end{split}
\end{equation*}
with boundary conditions
\begin{equation*}
    \begin{split}
    \alpha(0) = \alpha(1) = \beta(0) = 0,\\
    \alpha(x)\beta(1) = \sin(2\pi x).
    \end{split}
\end{equation*}

Setting $\beta(1)$ to $1$ yields $\alpha(x) = \sin(2\pi x)$, so that $\alpha''(x) = -4\pi^2\alpha(x)$ where $y = 1$, we find that $c = -4\pi^2$.
Solving the equation for $\beta(y)$, we find that
\begin{equation*}
    \beta(y) = b_1 e^{\sqrt{c} y} + b_2 e^{-\sqrt{c} y}.
\end{equation*}
Inserting $c = 4\pi$ and the boundary condtitions $\beta(0) = 0$ and $\beta(1) = 1$, we get
\begin{equation*}
    \beta(y) = \frac{\sinh(2\pi y)}{\sinh(2\pi)},
\end{equation*}
and finally
\begin{equation*}
    u(x,y) = \frac{\sin(2\pi x) \sinh(2\pi y)}{\sinh(2\pi)}.
\end{equation*}
