\section{Biharmonic equation}
\label{sec:PDE}

\newtheorem{theorem}{Theorem}
\newtheorem{lemma}{Lemma}

Consider teh inhomogeneous Biharmonic equation with clamped boundary conditions on the unit square $\Omega = [0, 1]^2$:
\begin{subequations}\label{eq:PDE}
  \begin{equation}
    \nabla^4 u = f \quad, (x, y) \in \Omega,
  \end{equation}
  \begin{equation}
    u = 0, \nabla^2u = 0 \quad, (x, y) \in \partial\Omega.
  \end{equation}
\end{subequations}

Firstly, note that the functions
$$
\sin(m \pi x) \sin(n \pi y), \quad m,n = 1, 2, \dots
$$
represent a complete basis for functions on $\Omega = [0, 1]^2$ with a boundary value of 0.
(Which is easily seen from the fact that the fourier series consist of such a set, and that for the given boundary condition, the coefficients of terms involving cosines and constant functions must be zero)
(TODO: comment on how to obtain this with separation of variables?)
Thus, for any function $u$ that has $u = 0$ on $\del\Omega$, we must be able to write
$$
u(x, y) =
\sum_{m=1}^\infty
\sum_{n=1}^\infty
F_{mn}
\sin(m\pi x)
\sin(n\pi y).
$$
Inserting the expression into the Biharmonic equation, we get, after acting on the expression with $\nabla^4$
\begin{align}
  \nabla^4 u &=
  \sum_{m=1}^\infty
  \sum_{n=1}^\infty
  F_{mn}
  \nabla^4
  \sin(m\pi x)\sin(n\pi y)\\
  &=
  \sum_{m=1}^\infty
  \sum_{n=1}^\infty
  F_{mn}
  \left(
  (m\pi)^4 + (n\pi)^4 + 2n^2m^2\pi^4
  \right)
  \sin(m\pi x)\sin(n\pi y)
  &= f.
\end{align}
(TODO: write as $((m\pi)^2+(n\pi)^2)^2$?)

Thus, with
$$
f(x, y)
=
\sum_{m=1}^\infty
\sum_{n=1}^\infty
G_{mn}
\sin(m\pi x)\sin(n\pi y),
$$
we must have that
$$
F_{mn} =
\frac{
  G_{mn}
}{
  \left(
  (m\pi)^4 + (n\pi)^4 + 2n^2m^2\pi^4
  \right)
}
$$
(TODO: comment on orthogonal sine functions?)
Observe that choosing $f$ such that the series is finite, ie. only a finite number of $G_{mn}$ are non-zero, the expression collapses into a finite expression.

%% b)

We may transform \eqref{eq:PDE} into a system of Poisson equation by introducing $g = \nabla^2 u$,
\begin{align}\label{eq:PDE-poisson}
  \nabla^2g &= f,\\
  \nabla^2u &= g.
\end{align}


%% c)
We will consider here two approximations of $\nabla^2 u = f$, the five point stencil and nine point stencil, which we will denote $\nabla_5^2$ and $\nabla_9^2$.

\newcommand{\crossStencil}[5]{%
  \begin{tikzpicture}[scale=0.5,baseline=1mm, every node/.style={scale=0.7}]
    \draw node[below]{$#1$} (0,0) -- (0,2) node[above]{$#2$};
    \draw (-1, 1) node[left]{$#3$} -- (1, 1) node[right]{$#4$};
    \node[above right] at (0,1) {$#5$};
  \end{tikzpicture}
}

\newcommand{\xStencil}[4]{%
  \begin{tikzpicture}[scale=0.5,baseline=1mm, every node/.style={scale=0.7}]
    \draw node[below left]{$#1$} (0,0) -- (1.41, 1.41) node[above right]{$#2$};
    \draw (0, 1.41) node[above left]{$#3$} -- (1.41, 0) node[below right]{$#4$};
  \end{tikzpicture}
}

Written in stencil diagrams, the five point stencil is given as (TODO: $f$ or $g$ here?)
$$
u \left(\crossStencil{1}{1}{1}{1}{-4}\right) = h^2 f
$$
while the nine point stencil is given by
$$
u
\left(
\xStencil{\frac16}{\frac16}{\frac16}{\frac16}
+
\crossStencil{\frac23}{\frac23}{\frac23}{\frac23}{-\frac{10}{3}}
\right)
=
h^2
f
\left(
\crossStencil{\frac1{12}}{\frac1{12}}{\frac1{12}}{\frac1{12}}{\frac23}
\right).
$$

Using one of these stencils will give a system of equations which we can write as a matrix equation,
$$
AU = BF,
$$
where $A$ and $B$ are matricies, $U$ is the solution that we seek, and $F$ is the inhomogeneity.
More precisely $U$ is a flattened array which represents the solution $u$;
the flattening is such that the rows of two-dimensional version of $U$ are conserved.
Thus, the next element of a column at position $n$, is at position $n+N$ in the flattened array, where $N$ is the number of elements in a row.
We will now consider the structure of the matrix $A$ in more detail.

Thus, with our 2D $U$ begin 
$$
\tilde{U} =
\begin{bmatrix}
  u_{11} & u_{12} & u_{13}\\
  u_{21} & u_{22} & u_{23}\\
  & \vdots
\end{bmatrix}
=
\begin{bmatrix}
  \vec{u_1}\\
  \vec{u_2}\\
  \vdots
\end{bmatrix}
$$
we have our flattened vector
$$
U =
\begin{bmatrix}
  u_{11} & u_{12} & u_{13} & \dots & u_{21} & u_{22} & \dots
\end{bmatrix}^T
$$

We will now describe the structure of the matricies involved in the problem, starting with the simpler five point stencil.
We recognize that in $U$ neighbouring elements correspond to grid points that are left and right of each other, while the grid point up and down is the element N places before and after.
Thus, writing out the five point stencil $K2D$, we get a toeplitz and symmetric matrix, where the main diagonal has -4 and the $\pm 1$ and $\pm N$ off diagonals have 1.
We can compactley write this as
$$
K2D =
\begin{bmatrix}
  K & 0 \\
  0 & K & 0\\
  0 & 0 & K \\
  &&&\ddots
\end{bmatrix}
+
\begin{bmatrix}
  -2I & I & 0 &  \\
  I & -2I & I & 0 \\
  0 & I & -2I & I & 0 \dots\\
  \vdots&&&\ddots
\end{bmatrix}.
$$
where $I$ is the identity matrix and $K$ is the one dimensional central finite difference matrix,
$$
K =
\begin{bmatrix}
  -2 & 1 & 0 &  \\
  1 & -2 & 1 & 0 \\
  0 & 1 & -2 & 1 & 0 \dots\\
  \vdots&&&\ddots
\end{bmatrix}.
$$
Using the Kronecker product, this may be written as
$$
K2D = \verb|kron|(I, K) + \verb|kron|(K, I)
$$
(TODO: note how boundary conditions are incorporated with this matrix structure?)

The nine point stencil has a slightly more complicated structure.
The block structure of the nine point stencil is as follows:
$$
\begin{bmatrix}
  4Q - 36 I & Q \\
  Q & 4Q - 36 I & 4Q \\
  0 & Q & 4Q - 36 I & Q \\
  & & & \ddots
\end{bmatrix}
=
\begin{bmatrix}
  4Q & Q \\
  Q & 4Q & 4Q \\
  0 & Q & 4Q & Q \\
  & & & \ddots
\end{bmatrix}
-
36
\begin{bmatrix}
  I & 0 \\
  0 & I & 0 \\
  0 & 0 & I & 0 \\
  & & & \ddots
\end{bmatrix}
$$
Notice the interesting recursive structure.
(TODO: should it be $-36$ or $-6$?)

TODO: write/use somewhere the general result for tridiag matrix ($a$ on diag)
\begin{equation*}
	\lambda_k = a - 2 \sqrt{bc} \cos(\frac{k \pi}{N + 1})
\end{equation*}

We can also write the nine point stencil as a sum of a five point stencil, where we simply change the weights, another matrix taking care of the NE, NW, etc. points.

Let
\begin{equation}
  \Sigma =
  \frac{1}{\sqrt{6}}
  \begin{bmatrix}
    0 & 1  \\
    1 & 0 & 1 \\
      & 1 & 0 & 1 \\
      &   & 1 & 0 & \ddots\\
      &   &   & \ddots  & \ddots
  \end{bmatrix}
\end{equation}
be the TST matrix with ones on its off-diagonals and zero on the diagonal.
The nine point stencil is then
\begin{equation}
  K2D^{(9)} + \Sigma \otimes \Sigma. \quad \text{TODO: should it be} K2D^{(5)}?
\end{equation}

We find the eigenvalues of $K2D^{(9)}$ directly by substituting in the appropriate weights in our previous expression from the five point stencil.
The $\Sigma$ matrix must by its structure obviously have the same eigenvectors as $K$, and by substituting in the formula, interpreting the zero diagonal as a zero weight, we find that the eigenvalues of $\Sigma$ are
$$
\frac{2}{\sqrt{6}} \cos(\frac{k \pi}{N+1}).
\quad \text{TODO: minus?}
$$
The eigenvalues of the Kronecker product $A \otimes B$ is the product of the eigenvalues of $A$ and $B$.
(TODO: also use property that eigenvalue of Kronecker sum is the sum of eigenvalues?)
Thus, the eigenvalues of $\Sigma \otimes \Sigma$ are
$$
\frac46
\cos(\frac{k \pi}{N+1})
\cos(\frac{l \pi}{N+1}).
$$
The eigenvalues of the nine point stencil are thus
\begin{equation}
  -\frac{10}{3}
  + \frac43
  \left(
  \cos(\frac{k \pi}{N+1})
  + \cos(\frac{l \pi}{N+1})
  \right)
  +
  \frac46
  \cos(\frac{k \pi}{N+1})
  \cos(\frac{l \pi}{N+1}).
\end{equation}

%% Let us defne an infinity norm for convenience
\newcommand{\inorm}[1]{
\lVert #1 \rVert_\infty
}

\subsection{Stability and order of the five point stencil}
We will here prove that the five point stencil is of order 2, following the outline provided in the exercise.
\emph{TODO: stability?}

We will here use the five point stencil defined as
$$
U \left(\crossStencil{1}{1}{1}{1}{-4}\right)
$$
so that the poisson equation reads
$$
- U \left(\crossStencil{1}{1}{1}{1}{-4}\right) = f.
$$
We do this simply for convenience.\\

%% 1
\begin{lemma}\label{pde:lemma:max}
If $\nabla_5^2 f \geq 0$ on $\Omega$, then the maximum value of $f$ is attained on $\partial \Omega$, that is
$$
\max(f)_\Omega \leq \max(f)_{\partial \Omega}.
$$
\end{lemma}
\begin{proof}
Suppose the opposite is true,
$$
\max(f)_\Omega \geq \max(f)_{\partial \Omega}.
$$
Then, there is an internal grid point on which $f$ attains it maximal value.
We denote this point by $x_0$, and label its neighbouring points $x_i,\quad i = 1,2,3,4$.
Then
$$
4f(x_0) = \sum_{i=1}^4 f(x_i) - \nabla_5^2 f(x_0) \leq \sum_{i=1}^4 f(x_i) \leq 4 f(x_0),
$$
where the last inequality is attained from the fact that $x_0$ is assumed to be the maximal value of $f$.
As the RHS is equal to the LHS, the equality must hold throughout, and as $f(x_i) \leq f(x_0$ we must have that all the neighbouring values have the same value as $x_0$, $f(x_1) = f(x_2) = f(x_3) = f(x_4) = f(x_0)$.
Applying this same argument to each of the neighbours, and then to their neighbours and so on, we ultimately reach the conclusion that all internal points have the same value, and that the same value is also attained on $\partial \Omega$, and we thus have a contradiction.
\end{proof}

%% 2
\begin{lemma}\label{pde:lemma:bound}
If $v$ is a discrete function that equals zero on $\partial \Omega$, then
$$
\inorm{v} \leq \frac18 \inorm{\nabla_5^2 v}.
$$
\end{lemma}
\begin{proof}
Consider the function
$$
\phi = \frac14 [ (x-\frac12)^2 + (y-\frac12)^2 ],
$$
It has the properties that $0 \leq \phi \leq \frac18$ and $\nabla_5^2 \phi = 1$.
Let $\inorm{\nabla_5^2 v} = M$.
Then
$$
\nabla_5^2 (v + \phi M) = \nabla_5^2 v +  M \geq 0.
$$
By lemma \ref{pde:lemma:max} we have then that $\nabla_5^2 (v + \phi M)$ attains its maximum value on $\partial \Omega$.
Thus
$$
\inorm{v}
\leq \inorm{v + \phi M}
\leq \max_{\partial \Omega}(v + \phi M)
= \max_{\partial\Omega} (\phi M)
\leq \frac18 \inorm{\nabla_5^2 v}.
$$
\end{proof}

%% 3
\begin{theorem}
If $\nabla^2 u = f$ and $\nabla_5^2 v = f$, then
$$
\inorm{u - v} \leq Ch^4 \lvert D^4 v\rvert_\infty.
$$
\end{theorem}
\begin{proof}
By our previous lemma \ref{pde:lemma:bound}
$$
\inorm{u - v} \leq \frac18 \inorm{\nabla_5^2 (u  - v)}.
$$
By Taylor expanding $u(x + h, y)$ and $u(x - h, y)$ we get
$$
\frac{1}{h^2} \delta_x^2 u = \partial_x^2 u + C h^2 \partial_x^4,
$$
and similarly for $y$.
Therefore
\begin{align*}
  - \nabla_5^2 u
  &=\frac{1}{h^2} (\delta_x^2 + \delta_y^2) u\\
  &= (\partial_x^2 + \partial_y^2 + C_x h^2 \partial_x^4 + C_y h^2 \partial_y^4) u\\
  &= (\nabla^2 + C_x h^2 \partial_x^4 + C_y h^2 \partial_y^4) u\\
  &\leq \nabla^2 u + 2 \max(C_x h^2 \partial_x^4 u, C_y h^2 \partial_y^4 u)\\
  &= \nabla^2 u + C h^2 \max(\partial_x^4 u, \partial_y^4 u).
\end{align*}

We then have
$$
\inorm{\nabla_5^2 (u  - v)} = C h^2 \inorm{D^4 u},
$$
where we by $\inorm{D^4 u}$ mean $\inorm{\max(\partial_x^4 u, \partial_y^4 u)}$. TODO: is it supposed to be $v$?
\end{proof}


\subsection{Stability and order of the nine point stencil}
Our proof for the nine point stencil will follow the same structure as for the five point stencil.



\subsection{The Fast Poisson Solver}
We are to solve the equation
$$
A U = F.
$$
Assuming that the eigenvectors of $A$ are a complete set, we may write
$$
F = a_1 y_1 + a_2 y_2 + ...,
$$
where $y_1, y_2, \dots$ are the eigenvectors of $A$.
The solution $U$ is the of course
$$
U =
\frac{a_1}{\lambda_1} y_1
+ \frac{a_2}{\lambda_2} y_2
+ \dots,
$$
where $\lambda_i$ is the eigenvalue corresponding to $y_i$.
In general, however, this is not a viable way to solve the problem, as it requires knowing all the eigenvalues and eigenvectors, as well as finding the coefficients $a_i$.
However, for the set of eigenvectors in this problem, which are sines, we have a very efficient algorithm for computing the coefficients, the discrete fast sine transform.
We also have simple analytical expressions for the eigenvalues.

Written as matrix expressions
\begin{align}
  A U &= F\\
  S\Lambda S U &= F\\
  &\Rightarrow\\
  U &= S\Lambda^{-1} S F,
\end{align}
where we used the fact that $S^{-1} = S$.
Moreover, formulated more directly with regards to implementing the solver, we have that the solutin is
$$
U = IFST(FST(F) / \Lambda),
$$
where $IFST, FST$ are the inverse and normal fast sine tranform.
